adding coqsim stuff

Simulator/CoqSim/Eval.v
@@ -1,40 +1,54 @@
-Require Import Compare_dec List String.
-Import ListNotations.
+Require Import Compare_dec List String Streams FinFun.
+Import ListNotations Fin2Restrict.
 
 Require Import Kami.AllNotations.
+
 Require Import Kami.Simulator.CoqSim.Misc.
-Require Import Kami.Simulator.CoqSim.IO.
 Require Import Kami.Simulator.CoqSim.TransparentProofs.
+Require Import Kami.Simulator.CoqSim.SimTypes.
+Require Import Kami.Simulator.CoqSim.HaskellTypes.
+
+Section Eval.
+
+Variable Word : nat -> Type.
+Variable Vec : nat -> Type -> Type.
+Variable M : Type -> Type.
+
+Context `{IsWord Word}.
+Context `{IsVector Vec}.
+Context `{IOMonad Word Vec M}.
 
 Fixpoint eval_Kind(k : Kind) : Type :=
   match k with
   | Bool => bool
-  | Bit n => word n
+  | Bit n => Word n
   | Struct n ks fs => Tuple (fun i => eval_Kind (ks i))
-  | Array n k' => Vec (eval_Kind k') n
+  | Array n k' => Vec n (eval_Kind k')
   end.
 
-Definition print_BF(bf : BitFormat) : nat -> string :=
+Definition print_BF(bf : BitFormat){n} : Word n -> string :=
   match bf with
-  | Binary => nat_binary_string
-  | Decimal => nat_decimal_string
-  | Hex => nat_hex_string
+  | Binary => print_word_bin
+  | Decimal => print_word_dec
+  | Hex => print_word_hex
   end.
+
+Axiom cheat : forall {X},X.
 
 Fixpoint print_Kind(k : Kind)(ff : FullFormat k) : eval_Kind k -> string :=
   match ff with
   | FBool n _ => fun x => space_pad n (if x then "1" else "0")
-  | FBit n m bf => fun x => zero_pad m (print_BF bf (wordToNat x))
-  | FStruct n fk fs ffs => fun x => ("{" ++ String.concat "; " (vec_to_list (vec_map (fun '(str1,str2) => str1 ++ ":" ++ str2) (add_strings fs (tup_to_vec _ (fun i => print_Kind (ffs i)) x)))) ++ "}")%string
-  | FArray n k' ff' => fun x => ("[" ++ String.concat "; " (vec_to_list (vec_map (fun '(n,y) => nat_decimal_string n ++ "=" ++ print_Kind ff' y) (add_indices x))) ++ "]")%string (*fix*)
+  | FBit n m bf => fun x => (*zero_pad m*) (print_BF bf x)
+  | FStruct n fk fs ffs => fun x => ("{ " ++ String.concat "; " (v_to_list (vmap (fun '(str1,str2) => str1 ++ ":" ++ str2) (add_strings fs (tup_to_vec _ (fun i => print_Kind (ffs i)) x)))) ++ "; }")%string
+  | FArray n k' ff' => fun x => ("[" ++ String.concat "; " (List.map (fun i => nat_decimal_string (f2n i) ++ "=" ++ print_Kind ff' (index i x)) (getFins n)) ++ "; ]")%string
   end.
 
 Fixpoint Kind_eq{k} : eval_Kind k -> eval_Kind k -> bool :=
-  match k with
+  match k return eval_Kind k -> eval_Kind k -> bool with
   | Bool => Bool.eqb
-  | Bit n => @weqb n
+  | Bit n => weqb
   | Struct n ks fs => TupEq (fun i => eval_Kind (ks i)) (fun i => @Kind_eq (ks i))
-  | Array n k' => VecEq (@Kind_eq k')
+  | Array n k' => vec_eq (@Kind_eq k')
   end.
 
 Definition eval_FK(k : FullKind) :=
@@ -43,15 +57,41 @@ Definition eval_FK(k : FullKind) :=
   | NativeKind t _ => t
   end.
 
-Fixpoint rand_val(k : Kind) : IO (eval_Kind k) :=
+Notation "'do' x <- y ; cont" := (bind y (fun x => cont)) (at level 20).
+
+Fixpoint default_val(k : Kind) : eval_Kind k :=
+  match k return eval_Kind k with
+  | Bool => false
+  | Bit n => nat_to_word 0
+  | Struct n ks fs => mkTup (fun i => eval_Kind (ks i)) (fun i => default_val (ks i))
+  | Array n k' => make_vec (fun _ => default_val k')
+  end.
+
+Definition default_val_FK(k : FullKind) : eval_FK k :=
   match k with
+  | SyntaxKind k' => default_val k'
+  | NativeKind T t => t
+  end.
+
+Fixpoint rand_tuple{n} : forall ts : Fin.t n -> Type, (forall i, M (ts i)) -> M (Tuple ts) :=
+  match n with
+  | 0 => fun _ _ => ret tt
+  | S m => fun ts mxs => (
+      do x <- mxs Fin.F1;
+      do xs <- rand_tuple (fun j => ts (Fin.FS j)) (fun j => mxs (Fin.FS j));
+      ret (x,xs)
+      )
+  end.
+
+Fixpoint rand_val(k : Kind) : M (eval_Kind k) :=
+  match k return M (eval_Kind k) with
   | Bool => rand_bool
   | Bit n => rand_word n
   | Struct n ks fs => rand_tuple (fun i => eval_Kind (ks i)) (fun i => rand_val (ks i))
   | Array n k' => rand_vec (rand_val k')
   end.
 
-Fixpoint rand_val_FK(k : FullKind) : IO (eval_FK k) :=
+Fixpoint rand_val_FK(k : FullKind) : M (eval_FK k) :=
   match k with
   | SyntaxKind k' => rand_val k'
   | NativeKind k' c => ret c
@@ -69,24 +109,47 @@ Definition eval_CABool(op : CABoolOp) : list bool -> bool :=
   | Xor => fun xs => fold_left xorb xs false
   end.
 
-Definition eval_UniBit{m n}(op : UniBitOp m n) : word m -> word n :=
-  evalUniBit op.
+Definition eval_UniBit{m n}(op : UniBitOp m n) : Word m -> Word n :=
+  match op with
+  | Inv n => inv
+  | TruncLsb lsb msb => trunc_lsb
+  | TruncMsb lsb msb => trunc_msb
+  | UAnd n => uand
+  | UOr n => uor
+  | UXor n => uxor
+  end.
 
-Definition eval_BinBit{m n p}(op : BinBitOp m n p) : word m -> word n -> word p :=
-  evalBinBit op.
+Definition eval_BinBit{m n p}(op : BinBitOp m n p) : Word m -> Word n -> Word p :=
+  match op with
+  | Sub n => sub
+  | Div n => div
+  | Rem n => rem
+  | Sll n m => sll
+  | Srl n m => srl
+  | Sra n m => sra
+  | Concat msb lsb => concat
+  end.
 
-Definition eval_CABit{n}(op : CABitOp) : list (word n) -> word n :=
-  evalCABit op.
+Definition eval_CABit{n}(op : CABitOp) : list (Word n) -> Word n :=
+  match op with
+  | Add => add
+  | Mul => mul
+  | Band => band
+  | Bor => bor
+  | Bxor => bxor
+  end.
 
-Definition eval_BinBitBool{m n}(op : BinBitBoolOp m n) : word m -> word n -> bool :=
-  evalBinBitBool op.
+Definition eval_BinBitBool{m n}(op : BinBitBoolOp m n) : Word m -> Word n -> bool :=
+  match op with
+  | LessThan n => wltb
+  end.
 
 Fixpoint eval_ConstT{k}(e : ConstT k) : eval_Kind k :=
   match e with
   | ConstBool b => b
-  | ConstBit n w => w
+  | ConstBit n w => nat_to_word (wordToNat w)
   | ConstStruct n ks ss es => mkTup (fun i => eval_Kind (ks i)) (fun i => eval_ConstT (es i))
-  | ConstArray n k' es => mkVec (fun i => eval_ConstT (es i))
+  | ConstArray n k' es => make_vec (fun i => eval_ConstT (es i))
   end.
 
 Definition eval_ConstFullT{k} (e : ConstFullT k) : eval_FK k :=
@@ -100,212 +163,58 @@ Fixpoint eval_Expr{k}(e : Expr eval_Kind k) : eval_FK k :=
   | Var _ v => v
   | Const _ v => eval_ConstT v
   | UniBool op e => eval_UniBool op (eval_Expr e)
-  | CABool op es => eval_CABool op (map eval_Expr es)
+  | CABool op es => eval_CABool op (List.map eval_Expr es)
   | UniBit m n op e => eval_UniBit op (eval_Expr e)
   | BinBit m n p op e1 e2 => eval_BinBit op (eval_Expr e1) (eval_Expr e2)
-  | CABit n op es => eval_CABit op (map eval_Expr es)
+  | CABit n op es => eval_CABit op (List.map eval_Expr es)
   | BinBitBool m n op e1 e2 => eval_BinBitBool op (eval_Expr e1) (eval_Expr e2)
   | ITE _ p e1 e2 => eval_Expr (if eval_Expr p then e1 else e2)
   | Eq _ e1 e2 => Kind_eq (eval_Expr e1) (eval_Expr e2)
   | ReadStruct n ks ss e i => tup_index i _ (eval_Expr e)
   | BuildStruct n ks ss es => mkTup _ (fun i => eval_Expr (es i))
-  | ReadArray n m k v i => match lt_dec (wordToNat (eval_Expr i)) n with
-                           | left pf => vec_index (Fin.of_nat_lt pf) (eval_Expr v)
+  | ReadArray n m k v i => match lt_dec (word_to_nat (eval_Expr i)) n with
+                           | left pf => index (Fin.of_nat_lt pf) (eval_Expr v)
                            | right _ => eval_ConstT (getDefaultConst k)
                            end
-  | ReadArrayConst n k v i => vec_index i (eval_Expr v)
-  | BuildArray n k v => mkVec (fun i => eval_Expr (v i))
+  | ReadArrayConst n k v i => index i (eval_Expr v)
+  | BuildArray n k v => make_vec (fun i => eval_Expr (v i))
   end.
 
-Definition eval_SysT(s : SysT eval_Kind) : IO unit :=
+(* Fixpoint chop_word{n x} : Word (n * x) -> Vec n (Word x) :=
+  match n with
+  | 
+
+Fixpoint val_unpack'(k : Kind) : Word (size k) -> eval_Kind k.
+Proof.
+  induction k; simpl; intro e.
+  (* Bool *)
+  - exact (weqb e (nat_to_word 1)).
+  (* Word *)
+  - exact e.
+  (* Tup *)
+  - admit.
+  - 
+ *)
+
+
+Definition val_unpack(k : Kind) : Word (size k) -> eval_Kind k :=
+  fun w => eval_Expr (unpack _ (Const _ (ConstBit (natToWord _ (word_to_nat w))))).
+
+Definition eval_SysT(s : SysT eval_Kind) : M unit :=
   match s with
   | DispString s => print s
   | DispExpr k e ff => print (print_Kind ff (eval_Expr e))
   | Finish => exit
   end.
 
-Fixpoint eval_list_SysT(xs : list (SysT eval_Kind)) : IO unit :=
+Fixpoint eval_list_SysT(xs : list (SysT eval_Kind)) : M unit :=
   match xs with
   | [] => ret tt
   | s::ys => (
-      io_do _ <- eval_SysT s;
+      do _ <- eval_SysT s;
       eval_list_SysT ys
       )
   end.
 
-Section EvalAction.
+End Eval.
 
-Definition SimReg := (string * {x : _ & fullType eval_Kind x})%type.
-Definition SimRegs := list SimReg.
-
-Variable regs : SimRegs.
-
-Fixpoint mkProd(ts : list Type) : Type :=
-  match ts with
-  | [] => unit
-  | T::ts' => (T * mkProd ts')%type
-  end.
-
-Fixpoint return_meth(meth : string)(sig : Signature)(meths : list (string * Signature)) : mkProd (map (fun dec => eval_Kind (fst (snd dec)) -> IO (eval_Kind (snd (snd dec)))) meths) -> option (eval_Kind (fst (sig)) -> IO (eval_Kind (snd (sig)))).
- refine match meths return mkProd (map (fun dec => eval_Kind (fst (snd dec)) -> IO (eval_Kind (snd (snd dec)))) meths) -> option (eval_Kind (fst (sig)) -> IO (eval_Kind (snd (sig)))) with
-  | [] => fun _ => None
-  | dec::meths' => match string_sigb (meth,sig) dec with
-                   | left pf => fun fs => Some _
-                   | right _ => fun fs => return_meth meth sig meths' (snd fs)
-                   end
-  end.
-Proof.
-  assert (sig = snd dec).
-  rewrite <- pf; auto.
-  rewrite H.
-  exact (fst fs).
-Defined.
-
-Fixpoint eval_ActionT{k}(meths : list (string * Signature))(updates : SimRegs)(a : ActionT eval_Kind k)(fs : mkProd (map (fun dec => eval_Kind (fst (snd dec)) -> IO (eval_Kind (snd (snd dec)))) meths)){struct a} : IO (SimRegs * eval_Kind k).
-  refine match a with
-  | MCall meth s e cont => match return_meth meth s meths fs with
-                           | None => error ("Method " ++ meth ++ " not found")
-                           | Some f => (
-                                io_do v <- f (eval_Expr e);
-                                eval_ActionT _ meths updates (cont v) fs
-                                )
-                           end
-  | LetExpr k e cont => eval_ActionT _ meths updates (cont (eval_Expr e)) fs
-  | LetAction k a cont => (
-      io_do p <- eval_ActionT _ meths updates a fs;
-      eval_ActionT _ meths (fst p) (cont (snd p)) fs
-      )
-  | ReadNondet k cont => (
-      io_do v <- rand_val_FK k;
-      eval_ActionT _ meths updates (cont v) fs
-      )
-  | ReadReg r k cont => match lookup String.eqb r regs with
-                        | None => reg_not_found r
-                        | Some p => _
-                        end
-  | WriteReg r k e a => match lookup String.eqb r regs with
-                        | None => reg_not_found r
-                        | Some p => _
-                        end
-  | IfElse e k a1 a2 cont => let a := if (eval_Expr e) then a1 else a2 in (
-      io_do p <- eval_ActionT _ meths updates a fs;
-      eval_ActionT _ meths (fst p) (cont (snd p)) fs
-      )
-  | Sys ss a => (
-      io_do _ <- eval_list_SysT ss;
-      eval_ActionT _ meths updates a fs
-      )
-  | Return e => ret (updates, eval_Expr e)
-  end.
-Proof.
-  - destruct p.
-    destruct x.
-    * destruct k.
-      + destruct (Kind_dec2 k1 k).
-        ++ rewrite e in f.
-           exact (eval_ActionT _ meths updates (cont f) fs).
-        ++ exact (error "mismatch").
-      + exact (error "no natives").
-    * exact (error "no natives").
-  - destruct p as [x _].
-    destruct k.
-    * destruct x.
-      + destruct (Kind_dec2 k k1).
-        ++ exact (eval_ActionT _ meths ((r, existT _ (SyntaxKind k) (eval_Expr e))::updates) a fs).
-        ++ exact (error "mismatch").
-      + exact (error "no natives!!!!").
-    * exact (error "no natives").
-Defined.
-
-Fixpoint curried(X : Type)(ts : list Type) : Type :=
-  match ts with
-  | [] => X
-  | T::ts' => T -> curried X ts'
-  end.
-
-Fixpoint curry(X : Type)(ts : list Type) : (mkProd ts -> X) -> curried X ts :=
-  match ts return (mkProd ts -> X) -> curried X ts with
-  | [] => fun f => f tt
-  | T::ts' => fun f t => curry ts' (fun xs => f (t,xs))
-  end.
-
-End EvalAction.
-
-Fixpoint do_single_update(upd : SimReg)(regs : SimRegs) : SimRegs :=
-  match upd with
-  | (reg,v) => match regs with
-               | [] => []
-               | (reg',v')::regs' => if String.eqb reg reg' then (reg,v)::regs' else (reg',v')::do_single_update upd regs'
-               end
-  end.
-
-Definition do_updates(upds : SimRegs)(regs : SimRegs) : SimRegs :=
-  fold_right do_single_update regs upds.
-
-Definition foo meths := SimRegs -> mkProd (map (fun dec : string * (Kind * Kind) => eval_Kind (fst (snd dec)) -> IO (eval_Kind (snd (snd dec)))) meths) -> IO (SimRegs * eval_Kind Void).
-
-CoFixpoint eval_BaseModule_rr_aux(meths : list (string * Signature))(curr_regs : SimRegs)(rem_rules all_rules : list (foo meths)) : mkProd (map (fun dec : string * (Kind * Kind) => eval_Kind (fst (snd dec)) -> IO (eval_Kind (snd (snd dec)))) meths) -> IO unit :=
-  match rem_rules with
-  | [] => fun fs => bind (ret tt) (fun _ => eval_BaseModule_rr_aux curr_regs all_rules all_rules fs)
-  | a::xs => fun fs => (
-      io_do p <- a curr_regs fs;
-      eval_BaseModule_rr_aux (do_updates (fst p) curr_regs) xs all_rules fs
-      )
-  end.
-
-
-Definition initialize_SimRegs(regs : list RegInitT) : SimRegs :=
-  map (fun '(r,existT k v) => match v return SimReg with
-                              | None => (r,existT _ k (eval_ConstFullT (getDefaultConstFullKind k)))
-                              | Some c => (r,existT _ k (eval_ConstFullT c))
-                              end) regs.
-
-Definition mkActionT : RuleT -> ActionT eval_Kind Void :=
-  fun '(_,a) => a eval_Kind.
-
-Definition eval_BaseModule_rr_unc(meths : list (string * Signature))(m : BaseModule) :=
-  match m with
-  | BaseRegFile _ => fun _ => error "BaseRegFile not supported"
-  | BaseMod regs rules _ => let all_rules := map (fun r rgs fs => @eval_ActionT rgs Void meths [] (mkActionT r) fs) rules in eval_BaseModule_rr_aux (initialize_SimRegs regs) all_rules all_rules
-  end.
-
-Definition eval_BaseModule_rr meths m := curry _ (eval_BaseModule_rr_unc meths m).
-
-Require Import Kami.Tutorial.SyntaxEx.
-
-Section BigTest.
-
-Definition sigs := [("extMeth1",(Bit 20, Bool));("extMeth2",(Bit 20,Void));("extMeth3",(Void,Bit 4));("extMeth4",(Void,Void));("extMeth2_2",(Bit 20, Void))].
-
-Definition out := eval_BaseModule_rr sigs (exampleModule "test").
-
-Ltac mycbv x := let y := (eval cbv [x eval_BaseModule_rr eval_BaseModule_rr_aux eval_ActionT lookup fst find fullType Bool.eqb snd Datatypes.length curried
-  eval_list_SysT eval_SysT eval_Expr string_sigb eq_trans f_equal
-  Signature_decb String.eqb Ascii.eqb andb Kind_decb Nat.eqb
-  eq_rect_r eq_rect eq_sym orb projT1 projT2 lt_dec tup_index Fin_forallb Signature_dec2 string_dec2 Kind_dec2 Kind_decb_eq2
-  string_rec String_eqb_eq2 string_ind Kind_ind Ascii_eqb_eq2 ascii_dec Nat_eqb_eq2 Nat_eqb_refl2 nth_Fin' curry] in x) in
-  let z := eval simpl in y in
-  let w := eval cbv [eq_rect_r eq_rect eq_sym nth_Fin' nth_Fin cast Datatypes.length eq_add_S f_equal] in z in
-  let v := eval simpl in w in
-   exact w.
-
-Definition out2 := ltac:(mycbv out).
-
-End BigTest.
-
-Require Import ExtrHaskellBasic.
-Extraction Language Haskell.
-
-Extract Inductive IO => "Prelude.IO"
-
-  [
-    "Prelude.putStrLn"
-    "Prelude.return"
-    "(GHC.Base.>>=)"
-    "Prelude.error"
-    "Prelude.return (unsafeCoerce Prelude.True)" (*fix*)
-    "Prelude.return (unsafeCoerce 0)"    (*fix*)
-    "System.Exit.exitSuccess"
-  ]
-
-  "Prelude.error ""Pattern matching on IO not supported""".
