Simulator/CoqSim/RegisterFile.v
@@ -1,0 +1,298 @@
+Require Import String.
+Require Import FinFun.
+
+Require Import Kami.AllNotations.
+Require Import Kami.Syntax.
+
+Require Import Kami.Simulator.CoqSim.Misc.
+Require Import Kami.Simulator.CoqSim.Eval.
+Require Import Kami.Simulator.CoqSim.SimTypes.
+
+Section RegFile.
+
+Context {V : nat -> Type -> Type}.
+Context `{IsVector V}.
+
+Context {W : nat -> Type}.
+Context `{IsWord W}.
+
+Context {M : Type -> Type}.
+Context `{StringMap M}.
+
+Context {IO : Type -> Type}.
+Context `{IOMonad W V IO}.
+
+Definition Val k := eval_Kind W V k.
+Definition ValFK k := eval_FK W V k.
+
+Inductive FileCall :=
+  | AsyncRead : FileCall
+  | ReadReq : string -> FileCall
+  | ReadResp : string -> FileCall
+  | WriteFC : FileCall.
+
+Inductive FileUpd :=
+  | IntRegWrite : string -> {k : Kind & Val k} -> FileUpd
+  | ArrWrite : string -> forall k, list (nat * Val k) -> FileUpd.
+
+Record RegFile := {
+  file_name : string;
+  is_wr_mask : bool;
+  chunk_size : nat;
+  readers : RegFileReaders;
+  write : string;
+  size : nat;
+  kind : Kind;
+  arr : V size (Val kind)
+  }.
+
+Record FileState := {
+  methods : M (FileCall * string);
+  int_regs : M {k : Kind & Val k};
+  files : M RegFile;
+  }.
+
+Definition empty_state : FileState := {|
+  methods := empty;
+  int_regs := empty;
+  files := empty
+  |}.
+
+Definition file_async_read(file : RegFile)(i : nat) : Val (Array (chunk_size file) (kind file)) :=
+  slice i _ (arr file).
+
+Definition isAddr(file : RegFile) : bool :=
+  match readers file with
+  | Sync isAddr _ => isAddr
+  | _ => false
+  end.
+
+Definition file_sync_readreq(val : {k : Kind & Val k})(file : RegFile)(regName : string) : option {k : Kind & Val k}. refine
+  match readers file with
+  | Async _ => None
+  | Sync true _ => if Kind_decb (projT1 val) (Bit (Nat.log2_up (size file))) then Some val else None
+  | Sync false _ => _
+  end.
+Proof.
+  (* isAddr = false *)
+  destruct val as [k v].
+  destruct (Kind_decb k (Bit (Nat.log2_up (size file)))) eqn:Keq.
+  - rewrite Kind_decb_eq in Keq.
+    rewrite Keq in v.
+    apply Some.
+    exists (Array (chunk_size file) (kind file)).
+    exact (slice (word_to_nat v) (chunk_size file) (arr file)).
+  - exact None.
+Defined.
+
+Axiom cheat : forall {X},X.
+
+Definition file_sync_readresp(state : FileState)(file : RegFile)(regName : string) : option (Val (Array (chunk_size file) (kind file))). refine
+  match map_lookup (M := M) regName (int_regs state) with
+  | None => None
+  | Some (existT k v) =>
+      match readers file with
+      | Async _ => None
+      | Sync true _ => _
+      | Sync false _ => _
+      end
+  end.
+Proof.
+  (* isAddr = true *)
+  - destruct (Kind_decb k (Bit (Nat.log2_up (size file)))) eqn:Keq.
+    * rewrite Kind_decb_eq in Keq.
+      rewrite Keq in v.
+      exact (Some (slice (word_to_nat v) (chunk_size file) (arr file))).
+    * exact None.
+  (* isAddr = false *)
+  - destruct (Kind_decb k (Array (chunk_size file) (kind file))) eqn:Keq.
+    * rewrite Kind_decb_eq in Keq.
+      rewrite Keq in v.
+      exact (Some v).
+    * exact (Some cheat).
+Defined.
+
+Definition file_writes_mask(file : RegFile)(i : nat)(mask : Val (Array (chunk_size file) Bool))(vals : Val (Array (chunk_size file) (kind file))) : list (nat * Val (kind file)) :=
+  let mask_indices := filter (fun i => index i mask) (getFins _) in
+    map (fun j => (i + Fin2Restrict.f2n j, index j vals)) mask_indices.
+
+Definition file_writes_no_mask(file : RegFile)(i : nat)(vals : Val (Array (chunk_size file) (kind file))) : list (nat * Val (kind file)) :=
+  map (fun j => (i + Fin2Restrict.f2n j, index j vals)) (getFins _).
+
+Definition void_nil : {k : Kind & Val k} :=
+  existT _ (Bit 0) (nat_to_word 0).
+
+Definition coerce(v : {k : Kind & Val k})(k : Kind) : option (Val k).
+  refine
+    match v with
+    | existT k' v' => _
+    end.
+Proof.
+  destruct (Kind_dec k k').
+  * rewrite e. exact (Some v').
+  * exact None.
+Defined.
+
+Fixpoint Tup_lookup{n} : forall (i : Fin.t n)(ks : Fin.t n -> Kind), Tuple (fun i => Val (ks i)) -> {k : Kind & Val k} :=
+  match n return forall (i : Fin.t n)(ks : Fin.t n -> Kind), Tuple (fun i => Val (ks i)) -> {k : Kind & Val k} with
+  | 0 => fun i => case0 _ i
+  | S m => fun i ks X => fin_case i _ (existT _ (ks F1) (fst X)) (fun j => (Tup_lookup  j _ (snd X)))
+  end.
+
+Definition  rf_methcall(state : FileState)(methName : string)(val : {k : Kind & Val k}) : option (option FileUpd * {k : Kind & Val k}). refine
+  match map_lookup methName (methods state) with
+  | None => None
+  | Some (fc, fileName) => match map_lookup fileName (files state) with
+                           | None => None
+                           | Some file => match fc with
+                                          | AsyncRead => _
+                                          | ReadReq regName => match file_sync_readreq val file regName with
+                                                               | None => None
+                                                               | Some p => Some (Some (IntRegWrite regName p), void_nil)
+                                                               end
+                                          | ReadResp regName => match file_sync_readresp state file regName with
+                                                                | None => None
+                                                                | Some v => Some (None, existT _ _ v)
+                                                                end
+                                          | WriteFC => match is_wr_mask file with
+                                                       | true => _
+                                                       | false => _
+                                                       end
+                                          end
+                           end
+  end.
+Proof.
+  (* AsyncRead *)
+  - destruct val as [k v].
+    destruct k eqn:G.
+    + exact None.
+    + pose (i := word_to_nat v).
+      exact (Some (None, existT _ _ (file_async_read file i))).
+    + exact None.
+    + exact None.
+  (* WriteFC is_wr_mask = true *)
+  - destruct val as [k v].
+    destruct k eqn:G.
+    + exact None.
+    + exact None.
+    + destruct n as [|[|[|]]]; [exact None | exact None | exact None | idtac]. (* n should be 3 *)
+      exact (let addr := Tup_lookup F1 k0 v in
+             let data_k := Tup_lookup (FS F1) k0 v in
+             let mask := Tup_lookup (FS (FS F1)) k0 v in
+             o_do addr' <- coerce addr (Bit (Nat.log2_up (size file)));
+             o_do data' <- coerce data_k (Array (chunk_size file) (kind file));
+             o_do mask' <- coerce mask (Array (chunk_size file) Bool);
+             o_ret (Some (ArrWrite fileName _ (file_writes_mask file (word_to_nat addr') mask' data')), void_nil)).
+    + exact None.
+  (* WriteFC is_wr_mask = false *)
+  - destruct val as [k v].
+    destruct k eqn:G.
+    + exact None.
+    + exact None.
+    + destruct n as [|[|]]; [exact None | exact None | idtac]. (* n should be 2 *)
+      exact (let addr := Tup_lookup F1 k0 v in
+             let data_k := Tup_lookup (FS F1) k0 v in
+             o_do addr' <- coerce addr (Bit (Nat.log2_up (size file)));
+             o_do data' <- coerce data_k (Array (chunk_size file) (kind file));
+             o_ret (Some (ArrWrite fileName _ (file_writes_no_mask file (word_to_nat addr') data')), void_nil)).
+    + exact None.
+Defined.
+
+Definition exec_file_update(u : FileUpd)(state : FileState) : FileState. refine
+  match u with
+  | IntRegWrite regName v =>
+    {| methods := methods state;
+       int_regs := insert regName v (int_regs state);
+       files := files state
+    |}
+  | ArrWrite fileName k upds => 
+    {| methods := methods state;
+       int_regs := int_regs state;
+       files := match map_lookup fileName (files state) with
+                | None => files state
+                | Some file => match Kind_dec k (kind file) with
+                               | left pf => insert fileName 
+                                    {|
+                                      file_name := file_name file;
+                                      is_wr_mask := is_wr_mask file;
+                                      chunk_size := chunk_size file;
+                                      readers := readers file;
+                                      write := write file;
+                                      size := size file;
+                                      kind := kind file;
+                                      arr := updates (arr file) _
+                                    |} (files state)
+                               | right _ => files state
+                               end
+                end
+    |}
+  end.
+Proof.
+  rewrite pf in upds.
+  exact upds.
+Defined.
+
+Definition exec_file_updates := List.fold_right exec_file_update.
+
+Axiom parseFile : forall (size idxNum : nat)(filepath : string), IO (V idxNum (W size)).
+
+Definition initialize_file(args : list (string * string))(rfb : RegFileBase)(state : FileState) : IO FileState :=
+
+  let array := match rfInit rfb with
+               | RFNonFile None => ret (make_vec (fun (_ : Fin.t (rfIdxNum rfb)) => default_val (rfData rfb)))
+               | RFNonFile (Some c) => ret (make_vec (fun _ => eval_ConstT c))
+               | RFFile isAscii isArg file _ _ _ =>
+                  let filepath := if isArg then match lookup String.eqb file args with
+                                               | Some fp => ret fp
+                                               | None => error ("File " ++ file ++ " not found!")
+                                               end else ret file in
+                  (io_do path <- filepath;
+                   io_do words <- parseFile (Syntax.size (rfData rfb)) (rfIdxNum rfb) path;
+                   ret (vec_map (@val_unpack W V _ _ _) words))
+               end in
+ (
+  io_do new_arr <- array;
+
+  let rf := {|
+                file_name := rfDataArray rfb;
+                is_wr_mask := rfIsWrMask rfb;
+                chunk_size := rfNum rfb;
+                readers := rfRead rfb;
+                write := rfWrite rfb;
+                size := rfIdxNum rfb;
+                kind := rfData rfb;
+                arr := new_arr
+            |} in
+
+  let reads := match rfRead rfb with
+               | Async rs => map (fun r => (r, (AsyncRead, rfDataArray rfb))) rs
+               | Sync b rs => map (fun r => (readReqName r, (ReadReq (readRegName r), rfDataArray rfb))) rs ++
+                              map (fun r => (readResName r, (ReadResp (readRegName r), rfDataArray rfb))) rs
+               end in
+
+  let newmeths := (rfWrite rfb, (WriteFC, rfDataArray rfb)) :: reads in
+  
+  let newvals := match rfRead rfb with
+                 | Async _ => []
+                 | Sync b rs => let k := if b then Bit (Nat.log2_up (rfIdxNum rfb)) else rfData rfb in
+                     map (fun r => (readRegName r, existT _ k (default_val k))) rs
+                 end in 
+
+  ret {|
+    methods := fold_right (fun '(x,y) st => insert x y st) (methods state) newmeths;
+    int_regs := fold_right (fun '(x,y) st => insert x y st) (int_regs state) newvals;
+    files := insert (rfDataArray rfb) rf (files state)
+    |}
+  ).
+
+Fixpoint initialize_files(args : list (string * string))(rfbs : list RegFileBase) : IO FileState :=
+  match rfbs with
+  | [] => ret empty_state
+  | (file::files) => (
+      io_do st <- initialize_files args files;
+      initialize_file args file st)
+  end.
+
+End RegFile.
+
+Extract Constant parseFile => "ParseExtract.parseFile".
