Simulator/CoqSim/SimTypes.v
@@ -1,0 +1,64 @@
+Require Import String Fin Kami.All.
+
+Class StringMap (M : Type -> Type) := {
+  empty : forall {V}, M V;
+  map_lookup : forall {V}, string -> M V -> option V;
+  insert : forall {V}, string -> V -> M V -> M V
+  }.
+
+Class IsVector (V : nat -> Type -> Type) := {
+  index : forall {X n}, Fin.t n -> V n X -> X;
+  vec_map : forall {X Y n}, (X -> Y) -> V n X -> V n Y;
+  vec_eq : forall {X n}, (X -> X -> bool) -> V n X -> V n X -> bool;
+  vec_to_list : forall {X n}, V n X -> list X;
+  make_vec : forall {X n}, (Fin.t n -> X) -> V n X;
+  slice : forall {X n} (i m : nat), V n X -> (V m X);
+  updates : forall {X n}, V n X -> list (nat * X) -> V n X
+  }.
+
+Class IsWord (W : nat -> Type) := {
+  inv : forall {m}, W m -> W m;
+  trunc_lsb : forall {m n}, W (m + n) -> W m;
+  trunc_msb : forall {m n}, W (m + n) -> W n;
+  uand : forall {m}, W m -> W 1;
+  uor : forall {m}, W m -> W 1;
+  uxor : forall {m}, W m -> W 1;
+
+  sub : forall {m}, W m -> W m -> W m;
+  div : forall {m}, W m -> W m -> W m;
+  rem : forall {m}, W m -> W m -> W m;
+  sll : forall {m n}, W m -> W n -> W m;
+  srl : forall {m n}, W m -> W n -> W m;
+  sra : forall {m n}, W m -> W n -> W m;
+  concat : forall {m n}, W m -> W n -> W (n + m);
+
+  add : forall {m}, list (W m) -> W m;
+  mul : forall {m}, list (W m) -> W m;
+  band : forall {m}, list (W m) -> W m;
+  bor : forall {m}, list (W m) -> W m;
+  bxor : forall {m}, list (W m) -> W m;
+
+  wltb : forall {m}, W m -> W m -> bool;
+
+  weqb : forall {m}, W m -> W m -> bool;
+
+  word_to_nat : forall {m}, W m -> nat;
+  nat_to_word : forall {m}, nat -> W m;
+  
+  print_word_bin : forall {m}, W m -> string;
+  print_word_dec : forall {m}, W m -> string;
+  print_word_hex : forall {m}, W m -> string
+  }.
+
+Class IOMonad{W V}`{IsWord W, IsVector V} (M : Type -> Type) := {
+  ret : forall {X}, X -> M X;
+  bind : forall {X Y}, M X -> (X -> M Y) -> M Y;
+  error : forall {X}, string -> M X;
+  print : string -> M unit;
+  rand_bool : M bool;
+  rand_word : forall n, M (W n);
+  rand_vec : forall {X n}, M X -> M (V n X);
+  exit : forall {X}, M X;
+  }.
+
+Notation "'io_do' x <- y ; cont" := (bind y (fun x => cont)) (at level 20).
