Simulator/CoqSim/Simulator.v
@@ -1,0 +1,375 @@
+Require Import Streams.
+
+Require Import Kami.AllNotations.
+
+Require Import Kami.Simulator.CoqSim.Misc.
+Require Import Kami.Simulator.CoqSim.TransparentProofs.
+Require Import Kami.Simulator.CoqSim.SimTypes.
+Require Import Kami.Simulator.CoqSim.HaskellTypes.
+Require Import Kami.Simulator.CoqSim.RegisterFile.
+Require Import Kami.Simulator.CoqSim.Eval.
+
+Section EvalAction.
+
+Variable Word : nat -> Type.
+Variable Vec : nat -> Type -> Type.
+Variable Map : Type -> Type.
+Variable M : Type -> Type.
+
+Context `{IsWord Word}.
+Context `{IsVector Vec}.
+Context `{StringMap Map}.
+Context `{IOMonad Word Vec M}.
+
+Notation "'do' x <- y ; cont" := (bind y (fun x => cont)) (at level 20).
+
+(* Variable KindInfo : Map string FullKind 
+Hypothesis ActionGood: forall Write r k in a, KindInfo r = k /\ forall Read r k in a, KindInfo r = k
+Lemma: SimRegGood: (r, k) in SimReg -> KindInfo r = k
+Theorem: ActionSimRegGood: forall Write r k in a, (r, k') in SimReg -> k = k' *)
+
+Definition eval_K := eval_Kind Word Vec.
+
+Definition eval_E := @eval_Expr Word Vec _ _.
+
+Definition SimReg := (string * {x : _ & fullType eval_K x})%type.
+Definition SimRegs := list SimReg.
+
+Section Regs.
+
+Variable regs : SimRegs.
+
+Record Update := {
+  reg_name : string;
+  kind : FullKind;
+  old_val : fullType eval_K kind;
+  new_val : fullType eval_K kind;
+  lookup_match : lookup String.eqb reg_name regs = Some (existT _ kind old_val)
+  }.
+
+Definition Updates := list Update.
+Definition FileUpdates := list (@FileUpd Vec Word).
+
+Fixpoint mkProd(ts : list Type) : Type :=
+  match ts with
+  | [] => unit
+  | T::ts' => (T * mkProd ts')%type
+  end.
+
+Class Environment E := {
+  envPre  : E -> FileState (V := Vec) (W := Word) (M := Map) -> SimRegs -> string -> M E;
+  envPost : E -> FileState (V := Vec) (W := Word) (M := Map) -> SimRegs -> string -> M E
+  }.
+
+Definition meth_sig{E}`{Environment E}(sig : Signature) : Type :=
+  eval_K (fst sig) -> FileState (V := Vec) (W := Word) (M := Map) -> SimRegs -> E -> M (E * (eval_K (snd sig))).
+
+Definition dec_sig{E}`{Environment E}(dec : string * Signature) : Type :=
+  meth_sig (snd dec).
+
+Fixpoint return_meth{E}`{Environment E}(meth : string)(sig : Signature)(meths : list (string * Signature)) : mkProd (List.map dec_sig meths) -> option (meth_sig sig).
+ refine match meths return mkProd (List.map dec_sig meths) -> option (meth_sig sig) with
+  | [] => fun _ => None
+  | dec::meths' => match string_sigb (meth,sig) dec with
+                   | left pf => fun fs => Some _
+                   | right _ => fun fs => return_meth _ _ meth sig meths' (snd fs)
+                   end
+  end.
+Proof.
+  assert (sig = snd dec).
+  rewrite <- pf; auto.
+  rewrite H6.
+  exact (fst fs).
+Defined.
+
+Definition reg_not_found{X} : string -> M X :=
+  fun reg => error ("register " ++ reg ++ " not found.").
+
+Fixpoint wf_action{k}(a : ActionT eval_K k) : Prop :=
+  match a with
+  | MCall meth s e cont => forall x, wf_action (cont x)
+  | LetExpr k e cont => forall x, wf_action (cont x)
+  | LetAction k a cont => (wf_action a /\ forall x, wf_action (cont x))
+  | ReadNondet k cont => forall x, wf_action (cont x)
+  | ReadReg r k' cont => match lookup String.eqb r regs with
+                         | None => False
+                         | Some (existT k'' _) => k' = k'' /\ forall x, wf_action (cont x)
+                         end
+  | WriteReg r k' e a => match lookup String.eqb r regs with
+                         | None => False
+                         | Some (existT k'' _) => k' = k'' /\ wf_action a
+                         end
+  | IfElse e k1 a1 a2 cont => (wf_action a1 /\ wf_action a2 /\ forall x, wf_action (cont x))
+  | Sys _ a => wf_action a
+  | Return _ => True
+  end.
+
+Fixpoint eval_ActionT{k}{E}`{Environment E}(env : E)(state : @FileState Vec Word Map)(meths : list (string * Signature))(updates : Updates)(fupdates : FileUpdates)(a : ActionT eval_K k)(a_wf : wf_action a)(fs : mkProd (List.map dec_sig meths)){struct a} : M (Updates * FileUpdates * eval_K k).
+  refine (match a return wf_action a -> _ with
+  | MCall meth s e cont => fun pf => 
+       match rf_methcall state meth (existT _ (fst s) (eval_E e)) with
+      | Some (o, existT k v) => match Kind_dec k (snd s) with
+                                | left _ => _
+                                | right _ => error ("Type mismatch")
+                                end
+      | None => match return_meth meth s meths fs with
+                | None => error ("Method " ++ meth ++ " not found")
+                | Some f => (
+                    do p <- f (eval_Expr e) state regs env;
+                    eval_ActionT _ _ _ (fst p) state meths updates fupdates (cont (snd p)) _ fs
+                    )
+                end
+      end
+  | LetExpr k e cont => fun pf => eval_ActionT _ _ _ env state meths updates fupdates (cont (eval_Expr e)) _ fs
+  | LetAction k a cont => fun pf => (
+      do p <- eval_ActionT _ _ _ env state meths updates fupdates a _ fs;
+      eval_ActionT _ _ _ env state meths (fst (fst p)) (snd (fst p)) (cont (snd p)) _ fs
+      )
+  | ReadNondet k cont => fun pf => (
+      do v <- rand_val_FK k;
+      eval_ActionT _ _ _ env state meths updates fupdates (cont v) _ fs
+      )
+  | ReadReg r k cont => fun pf=> match lookup String.eqb r regs with
+                        | None => reg_not_found r
+                        | Some p => _
+                        end
+  | WriteReg r k e a => fun pf => match lookup String.eqb r regs with
+                        | None => reg_not_found r
+                        | Some p => _
+                        end
+  | IfElse e k a1 a2 cont => fun pf => let a := if (eval_Expr e) then a1 else a2 in (
+      do p <- eval_ActionT _ _ _ env state meths updates fupdates a _ fs;
+      eval_ActionT _ _ _ env state meths (fst (fst p)) (snd (fst p)) (cont ((snd p))) _ fs
+      )
+  | Sys ss a => fun pf => (
+      do _ <- eval_list_SysT ss;
+      eval_ActionT _ _ _ env state meths updates fupdates a _ fs
+      )
+  | Return e => fun pf => ret (updates, fupdates, eval_Expr e)
+  end a_wf).
+Proof.
+  (* MCall *)
+  - rewrite e0 in v.
+    destruct o as [fupd|].
+    + exact (eval_ActionT _ _ _ env state meths updates (fupd::fupdates) (cont v) (pf _) fs).
+    + exact (eval_ActionT _ _ _ env state meths updates fupdates (cont v) (pf _) fs).
+  - apply pf.
+  - apply pf.
+  - apply pf.
+  - apply pf.
+  - apply pf.
+  
+  (* ReadReg *)
+  - destruct p.
+    simpl in pf.
+    destruct lookup in pf.
+    * destruct s; destruct pf as [keq pf'].
+      rewrite <- keq in f0.
+      exact (eval_ActionT _ _ _ env state meths updates fupdates (cont f0) (pf' _) fs).
+    * destruct pf.
+  (* WriteReg *)
+  - simpl in pf.
+    destruct lookup eqn:lk in pf.
+    * destruct s.
+      destruct pf as [keq pf'].
+      rewrite keq in e.
+      pose (upd := {|
+        reg_name := r;
+        kind := x;
+        old_val := f;
+        new_val := eval_Expr e;
+        lookup_match := lk
+        |}).
+      exact (eval_ActionT _ _ _ env state meths (upd::updates) fupdates a pf' fs).
+    * destruct pf.
+  - simpl in pf; destruct (eval_Expr e); tauto.
+  - apply pf.
+  - exact pf.
+Defined.
+
+Fixpoint curried(X : Type)(ts : list Type) : Type :=
+  match ts with
+  | [] => X
+  | T::ts' => T -> curried X ts'
+  end.
+
+Fixpoint curry(X : Type)(ts : list Type) : (mkProd ts -> X) -> curried X ts :=
+  match ts return (mkProd ts -> X) -> curried X ts with
+  | [] => fun f => f tt
+  | T::ts' => fun f t => curry ts' (fun xs => f (t,xs))
+  end.
+
+Definition eval_RuleT{E}`{Environment E}(env : E)(state : FileState)(meths : list (string * Signature))(r : RuleT)(r_wf : wf_action (snd r eval_K))(fs : mkProd (List.map dec_sig meths)) : M (Updates * FileUpdates * eval_K Void) :=
+  eval_ActionT env state meths [] [] ((snd r) eval_K) r_wf fs.
+
+Fixpoint do_single_update(upd : Update)(regs : SimRegs) : SimRegs :=
+  match regs with
+  | [] => []
+  | (reg',v')::regs' => if String.eqb (reg_name upd) reg' then (reg', existT _ (kind upd) (new_val upd))::regs' else (reg',v')::do_single_update upd regs'
+  end.
+
+Definition do_updates(upds : Updates)(regs : SimRegs) : SimRegs :=
+  fold_right do_single_update regs upds.
+
+End Regs.
+
+Section Regs2.
+
+Definition consistent(regs1 regs2 : SimRegs) := forall r k v,
+  lookup String.eqb r regs1 = Some (existT _ k v) -> exists v', lookup String.eqb r regs2 = Some (existT _ k v').
+
+Lemma consistent_refl : forall regs, consistent regs regs.
+Proof.
+  intros regs r k v lk.
+  exists v; auto.
+Qed.
+
+Lemma consistent_trans : forall regs1 regs2 regs3, consistent regs1 regs2 -> consistent regs2 regs3 -> consistent regs1 regs3.
+Proof.
+  intros regs1 regs2 regs3 cons12 cons23 r k v Hv.
+  destruct (cons12 r k v) as [v' Hv']; auto.
+  destruct (cons23 r k v') as [v'' Hv'']; auto.
+  exists v''; auto.
+Qed.
+
+Lemma lookup_cons : forall K V (eqb : K -> K -> bool) k k' v (ps : list (K*V)), lookup eqb k ((k',v)::ps) =
+  if eqb k k' then Some v else lookup eqb k ps.
+Proof.
+  intros.
+  unfold lookup.
+  unfold find.
+  simpl.
+  destruct (eqb k k'); auto.
+Qed.
+
+Lemma consistent_cons_cong : forall (regs1 regs2 : SimRegs)(r : SimReg), consistent regs1 regs2 -> consistent (r::regs1) (r::regs2).
+Proof.
+  intros regs1 regs2 r cons12 s k v Hv.
+  destruct r.
+  rewrite lookup_cons in Hv.
+  rewrite lookup_cons.
+  destruct (String.eqb s s0).
+  - exists v; auto.
+  - destruct (cons12 s k v); auto.
+    exists x; auto.
+Qed.
+
+(*
+Lemma consistent_do_update_cong : forall (regs1 regs2 : SimRegs)(upd : Update regs1),
+  consistent regs1 regs2 -> consistent (do_single_update upd regs1) (do_single_update upd regs2).
+Proof.
+Admitted.
+
+Lemma update_consistent : forall (regs : SimRegs)(upd : Update regs), consistent regs (do_single_update upd regs).
+Proof.
+  intros regs upd r k v Hv.
+  pose (lookup_match upd).
+  Print Update.
+*)
+
+Lemma wf_consistent_stable : forall {k} (a : ActionT eval_K k) regs1 regs2, consistent regs1 regs2 -> wf_action regs1 a -> wf_action regs2 a.
+Proof.
+  intros.
+  induction a; simpl.
+Admitted.
+
+Lemma updates_consistent : forall (regs : SimRegs)(upds : Updates regs), consistent regs (do_updates upds regs).
+Proof.
+  intros; induction upds; simpl.
+  - apply consistent_refl.
+  - apply (@consistent_trans _ (do_single_update a regs) _).
+Admitted.
+
+Lemma wf_updates_stable{k} : forall (regs : SimRegs)(upds : Updates regs)(a : ActionT eval_K k),
+  wf_action regs a -> wf_action (do_updates upds regs) a.
+Proof.
+  intros.
+  apply (@wf_consistent_stable _ _ regs).
+  - apply updates_consistent.
+  - auto.
+Qed.
+
+Definition maintain_wf{k} regs (upds : Updates regs) (a : ActionT eval_K k) : {r : RuleT & wf_action regs a} -> {r : RuleT & wf_action (do_updates upds regs) a}.
+Admitted.
+
+(* TODO: FIGURE OUT IF THE ENV NEEDS TO BE UPDATED AT SOME POINT *)
+Check envPre.
+Print RuleT.
+
+Fixpoint eval_Rules{E}`{Environment E}(env : E)(state : FileState (V := Vec) (W := Word) (M := Map))(timeout : nat)(meths : list (string * Signature))(init_regs : SimRegs)(rules : Stream {r : RuleT & wf_action init_regs (snd r eval_K)}){struct timeout} : mkProd (List.map dec_sig meths) -> M unit. refine
+  match timeout with
+  | 0 => fun fs => error "TIMEOUT"
+  | S timeout' => fun fs => match rules with
+                            | Cons r rules' => (
+                                do env' <- envPre env state init_regs (fst (projT1 r));
+                                do p <- eval_RuleT init_regs env' state meths (projT1 r) (projT2 r)  fs;
+                                do env'' <- envPost env' state init_regs (fst (projT1 r));
+                                eval_Rules _ _  env'' (exec_file_updates state (snd (fst p))) timeout' meths (do_updates (fst (fst p)) init_regs) (Streams.map _ rules') fs
+                                )
+                            end
+  end.
+Proof.
+  intros [rule wf].
+  exists rule.
+  apply wf_updates_stable; auto.
+Defined.
+
+Definition initialize_SimRegs(regs : list RegInitT) : SimRegs :=
+  List.map (fun '(r,existT k v) => match v return SimReg with
+                                   | None => (r,existT _ k (eval_ConstFullT (getDefaultConstFullKind k)))
+                                   | Some c => (r,existT _ k (eval_ConstFullT c))
+                                   end) regs.
+
+Lemma cons_neq{X}(x : X)(xs : list X) : x::xs <> [].
+Proof.
+  discriminate.
+Qed.
+
+Fixpoint wf_rules(regs : SimRegs)(rules : list RuleT) :=
+  match rules with
+  | [] => True
+  | r::rs => wf_action regs (snd r eval_K) /\ wf_rules regs rs
+  end.
+
+Definition wf_bm(basemod : BaseModule) : Prop :=
+  match basemod with
+  | BaseRegFile rf => False
+  | BaseMod regs rules dms => wf_rules (initialize_SimRegs regs) rules
+  end.
+
+Definition get_wf_rules : forall regs rules, wf_rules (initialize_SimRegs regs) rules -> 
+  list {r : RuleT & wf_action (initialize_SimRegs regs) (snd r eval_K)}.
+Proof.
+  intros.
+  induction rules.
+  - exact [].
+  - simpl in H5; destruct H5.
+    exact ((existT _ a H5)::IHrules H6).
+Defined.
+
+Definition eval_Basemodule_rr{E}`{Environment E}(env : E)(args : list (string * string))(rfbs : list RegFileBase)(timeout : nat)(meths : list (string * Signature))(basemod : BaseModule)(wf : wf_bm basemod) : mkProd (List.map dec_sig meths) -> M unit. refine (
+  match basemod return wf_bm basemod -> _ with
+  | BaseRegFile rf => fun pf fs => _
+  | BaseMod regs rules dms =>
+      match rules with
+      | [] => fun _ _ => error "empty rules"
+      | r::rs => fun pf fs => _ (* eval_Rules timeout meths (initialize_SimRegs regs) (unwind_list (r::rs) (@cons_neq _ r rs)) *)
+      end
+  end wf).
+Proof.
+  - destruct pf.
+  - unfold wf_bm in pf.
+    refine (do state <- initialize_files args rfbs;
+    eval_Rules env state timeout meths (initialize_SimRegs regs) (unwind_list (get_wf_rules _ _ pf) _) fs).
+    simpl.
+    destruct pf; discriminate.
+Defined.
+
+Definition eval_BaseMod{E}`{Environment E}(env : E)(args : list (string * string))(rfbs : list RegFileBase)(timeout : nat)(meths : list (string * Signature))(basemod : BaseModule)(wf : wf_bm basemod) :=
+  curry _ (eval_Basemodule_rr env args rfbs timeout meths basemod wf).
+
+End Regs2.
+
+End EvalAction.
+
+Definition eval_BaseMod_Haskell := @eval_BaseMod HWord HVec HMap IO _ _ _ _ _ _.
